comm/Flag.v
@@ -1,0 +1,25 @@
+From Coq Require Import List.
+Import ListNotations.
+
+Inductive bpf_flag: Type := 
+  | BPF_SUCC_RETURN         (**r =  1, *)
+  | BPF_OK                  (**r =  0, *)
+  | BPF_ILLEGAL_INSTRUCTION (**r = -1, *)
+  | BPF_ILLEGAL_MEM         (**r = -2, *)
+  | BPF_ILLEGAL_JUMP        (**r = -3, *)
+  | BPF_ILLEGAL_CALL        (**r = -4, *)
+  | BPF_ILLEGAL_LEN         (**r = -5, *)
+  | BPF_ILLEGAL_REGISTER    (**r = -6  *)
+  | BPF_NO_RETURN           (**r = -7, *)
+  | BPF_OUT_OF_BRANCHES     (**r = -8, *)
+  | BPF_ILLEGAL_DIV         (**r = -9, *)
+  | BPF_ILLEGAL_SHIFT       (**r = -10,*)
+  | BPF_ILLEGAL_ALU         (**r = -11,*)
+.
+Lemma bpf_flag_eq: forall (x y: bpf_flag), {x=y} + {x<>y}.
+Proof.
+decide equality. Defined.
+
+(** flag_eq: flag -> flag -> bool
+  *)
+Definition flag_eq (x y: bpf_flag): bool := if bpf_flag_eq x y then true else false.
