comm/List64.v
@@ -1,0 +1,25 @@
+From Coq Require Import List ZArith.
+Import ListNotations.
+
+From compcert.cfrontend Require Csyntax Ctypes Cop.
+From compcert.common Require Values.
+From compcert.lib Require Import Integers.
+
+
+Module MyList.
+
+  Definition t := list int64.
+  Definition index_s32 (l: t) (idx: int): int64 := 
+    List.nth (Z.to_nat (Int.signed idx)) l (Int64.zero).
+  Definition index_nat (l: t) (idx: nat): int64 := 
+    List.nth idx l (Integers.Int64.zero).
+
+End MyList.
+
+(** length of MyList should be a extern variable? *)
+
+Definition MyListType := MyList.t.
+Definition MyListIndexs32 := MyList.index_s32.
+Definition MyListIndexnat := MyList.index_nat.
+
+Definition default_list: MyListType :=  [].
