comm/MemRegion.v
@@ -1,0 +1,40 @@
+From Coq Require Import List ZArith.
+Import ListNotations.
+
+From compcert.cfrontend Require Csyntax Ctypes Cop.
+From compcert Require Import Integers Values Memtype.
+
+From bpf.comm Require Import rBPFMemType.
+
+Record memory_region : Type := mkmr{
+  start_addr : val;
+  block_size : val;   (**r should those be val32_t? *)
+  block_perm : permission; (**r let's say it should be u32 *)
+  block_ptr  : val;
+}.
+
+Definition default_memory_region := {|
+  start_addr := Vnullptr;
+  block_size := Vzero;
+  block_perm := Nonempty;
+  block_ptr  := Vnullptr;
+|}.
+
+Module Memory_regions.
+
+  Definition t := list memory_region.
+  Definition index_nat (l: t) (idx: nat): memory_region := 
+    List.nth idx l (default_memory_region).
+
+End Memory_regions.
+
+Definition MyMemRegionsType := Memory_regions.t.
+Definition MyMemRegionsIndexnat := Memory_regions.index_nat.
+
+Definition default_memory_regions: MyMemRegionsType :=  [].
+
+Fixpoint MyMemRegionsAdd (mr: memory_region) (l: MyMemRegionsType) :=
+  match l with
+  | [] => [mr]
+  | hd :: tl => hd :: MyMemRegionsAdd mr tl
+  end.
