comm/Monad.v
@@ -1,0 +1,56 @@
+From compcert Require Import AST Integers Values Memory.
+
+From bpf.comm Require Import Regs Flag MemRegion State.
+
+Definition M (A: Type) := state -> option (A * state).
+
+Definition returnM {A: Type} (a: A) : M A := fun st => Some (a, st).
+Definition errorM {A: Type} : M A := fun st => None.
+Definition bindM {A B: Type} (x: M A) (f: A -> M B) : M B :=
+  fun st =>
+    match x st with
+    | None => None
+    | Some (x', st') => (f x') st'
+    end.
+
+Definition eval_pc: M int := fun st => Some (eval_pc st, st).
+Definition upd_pc (p: int): M unit := fun st => Some (tt, upd_pc p st).
+Definition upd_pc_incr: M unit := fun st => Some (tt, upd_pc_incr st).
+
+Definition eval_flag: M bpf_flag := fun st => Some (eval_flag st, st).
+Definition upd_flag (f:bpf_flag) : M unit := fun st => Some (tt, upd_flag f st).
+
+Definition eval_mrs_num: M nat := fun st => Some (eval_mem_num st, st).
+
+Definition eval_reg (r: reg) : M val := fun st => Some (eval_reg r st, st).
+Definition upd_reg (r: reg) (v: val) : M unit := fun st => Some (tt, upd_reg r v st).
+
+Definition eval_mrs_regions : M MyMemRegionsType := fun st => Some (eval_mem_regions st, st).
+
+Definition eval_mem_regions: M MyMemRegionsType := fun st => Some (eval_mem_regions st, st).
+
+Definition eval_mem : M Mem.mem := fun st => Some (eval_mem st, st).
+
+
+Definition load_mem (chunk: memory_chunk) (ptr: val): M val := fun st => Some (load_mem chunk ptr st, st).
+
+Definition store_mem_imm (chunk: memory_chunk) (ptr: val) (v: val) : M unit := fun st => 
+  match store_mem_imm chunk ptr v st with
+  | Some res => Some (tt, res)
+  | None => None
+  end.
+
+Definition store_mem_reg (chunk: memory_chunk) (ptr: val) (v: val) : M unit := fun st => 
+  match store_mem_reg chunk ptr v st with
+  | Some res => Some (tt, res)
+  | None => None
+  end.
+
+Definition eval_ins_len : M int := fun st => Some (eval_ins_len st, st).
+Definition eval_ins (idx: int) : M int64 := fun st => Some (eval_ins idx st, st).
+
+Declare Scope monad_scope.
+Notation "'do' x <- a ; b" :=
+  (bindM a (fun x => b))
+    (at level 200, x name, a at level 100, b at level 200)
+  : monad_scope.
