comm/Regs.v
@@ -1,17 +1,11 @@
 From compcert.cfrontend Require Csyntax Ctypes Cop.
-From compcert.common Require Values Memory.
+From compcert.common Require Import Values Memory.
 From compcert.lib Require Import Integers.
-
-From dx Require Import ResultMonad IR.
-From dx.Type Require Bool Nat.
-
-From bpf.comm Require Import Regs.
-From bpf.src Require Import IdentDef CoqIntegers DxIntegers DxValues. (* GenMatchable.*)
 
 From Coq Require Import List ZArith.
 Import ListNotations.
 
-(*
+
 Inductive reg: Type :=
   | R0:reg | R1:reg | R2:reg
   | R3:reg | R4:reg | R5:reg
@@ -37,7 +31,7 @@ Record regmap: Type := make_regmap{
   r10_val : Values.val;
 }.
 
-Definition eval_regmap (r:reg) (regs:regmap): val64_t := 
+Definition eval_regmap (r:reg) (regs:regmap): val := 
   match r with
   | R0  => r0_val regs
   | R1  => r1_val regs
@@ -52,7 +46,7 @@ Definition eval_regmap (r:reg) (regs:regmap): val64_t :=
   | R10 => r10_val regs
   end.
 
-Definition upd_regmap (r:reg) (v:val64_t) (regs:regmap): regmap :=
+Definition upd_regmap (r:reg) (v:val) (regs:regmap): regmap :=
   match r with
   | R0  => 
     {|
@@ -210,6 +204,8 @@ Definition upd_regmap (r:reg) (v:val64_t) (regs:regmap): regmap :=
     |} 
   end.
 
+Definition val64_zero := Vlong Int64.zero.
+
 Definition init_regmap: regmap := {|
   r0_val  := val64_zero;
   r1_val  := val64_zero;
@@ -250,128 +246,11 @@ Definition z_to_reg (z:Z): reg :=
   else
     R10.
 
-Definition get_dst (i:int64_t):Z := Int64.unsigned (Int64.shru (Int64.and i int64_0xfff) int64_8).
-Definition get_src (i:int64_t):Z := Int64.unsigned (Int64.shru (Int64.and i int64_0xffff) int64_12).
+Definition get_dst (i:int64):Z := Int64.unsigned (Int64.shru (Int64.and i (Int64.repr 0xfff)) (Int64.repr 8)).
+Definition get_src (i:int64):Z := Int64.unsigned (Int64.shru (Int64.and i (Int64.repr 0xffff)) (Int64.repr 12)).
 
-Definition int64_to_dst_reg (ins: int64_t): reg :=
+Definition int64_to_dst_reg (ins: int64): reg :=
   z_to_reg (get_dst ins).
 
-Definition int64_to_src_reg (ins: int64_t): reg :=
+Definition int64_to_src_reg (ins: int64): reg :=
   z_to_reg (get_src ins).
-*)
-
-(******************** Dx Related *******************)
-
-(** Coq2C: reg -> unsigned int;
-           matchableType: R_i -> i,  i.e. R0 -> 0
-  *)
-
-Definition regCompilableType :=
-  MkCompilableType reg C_U32.
-
-Definition regSymbolType :=
-  MkCompilableSymbolType nil (Some regCompilableType).
-
-Definition Const_R0 := constant regSymbolType R0 C_U32_zero.
-
-Definition Const_R1 := constant regSymbolType R1 C_U32_one.
-
-Definition Const_R2 := constant regSymbolType R2 C_U32_2.
-
-Definition Const_R3 := constant regSymbolType R3 C_U32_3.
-
-Definition Const_R4 := constant regSymbolType R4 C_U32_4.
-
-Definition Const_R5 := constant regSymbolType R5 C_U32_5.
-
-Definition Const_R6 := constant regSymbolType R6 C_U32_6.
-
-Definition Const_R7 := constant regSymbolType R7 C_U32_7.
-
-Definition Const_R8 := constant regSymbolType R8 C_U32_8.
-
-Definition Const_R9 := constant regSymbolType R9 C_U32_9.
-
-Definition Const_R10 := constant regSymbolType R10 C_U32_10.
-
-Close Scope Z_scope.
-
-Definition int64ToregSymbolType :=
-  MkCompilableSymbolType [int64CompilableType] (Some regCompilableType).
-
-Definition Const_int64_to_dst_reg :=
-  MkPrimitive int64ToregSymbolType
-                int64_to_dst_reg
-                (fun es => match es with
-                           | [e1] => Ok (Csyntax.Ecast (Csyntax.Ebinop Cop.Oshr
-                                          (Csyntax.Ebinop Cop.Oand e1 C_U64_0xfff C_U64)
-                                          C_U64_8 C_U64) C_U32)
-                           | _       => Err PrimitiveEncodingFailed
-                           end).
-
-Definition Const_int64_to_src_reg :=
-  MkPrimitive int64ToregSymbolType
-                int64_to_src_reg
-                (fun es => match es with
-                           | [e1] => Ok (Csyntax.Ecast (Csyntax.Ebinop Cop.Oshr
-                                          (Csyntax.Ebinop Cop.Oand e1 C_U64_0xffff C_U64)
-                                          C_U64_12 C_U64) C_U32)
-                           | _       => Err PrimitiveEncodingFailed
-                           end).
-
-
-(** Coq2C: regmap -> unsigned long long int regmap[11];
-  *)
-Definition C_regmap: Ctypes.type := Ctypes.Tarray C_U64 11%Z Ctypes.noattr.
-
-Definition regmapCompilableType := MkCompilableType regmap C_regmap.
-
-(** Type signature: reg -> regmap -> val64
-  *)
-Definition regToregmapToVal64SymbolType :=
-  MkCompilableSymbolType [regCompilableType; regmapCompilableType] (Some val64CompilableType).
-
-Definition Const_eval_regmap :=
-  MkPrimitive regToregmapToVal64SymbolType
-                eval_regmap
-                (fun es => match es with
-                           | [e1; e2] => Ok (Csyntax.Eindex e2 e1 C_U64)
-                           | _       => Err PrimitiveEncodingFailed
-                           end).
-
-(** Type signature: reg -> val64 -> regmap -> regmap
-  *)
-Definition regToval64ToregmapToregmapSymbolType :=
-  MkCompilableSymbolType [regCompilableType; val64CompilableType; regmapCompilableType] (Some regmapCompilableType).
-
-Definition Const_upd_regmap :=
-  MkPrimitive regToval64ToregmapToregmapSymbolType
-                upd_regmap
-                (fun es => match es with
-                           | [r; v; regmap] => Ok (
-                              Csyntax.Eassign
-                              (Csyntax.Eindex regmap r C_U64)
-                              (Csyntax.Evalof v C_U64)
-                              C_U64)
-                           | _       => Err PrimitiveEncodingFailed
-                           end).
-
-Module Exports.
-  Definition regCompilableType      := regCompilableType.
-  Definition Const_R0               := Const_R0.
-  Definition Const_R1               := Const_R1.
-  Definition Const_R2               := Const_R2.
-  Definition Const_R3               := Const_R3.
-  Definition Const_R4               := Const_R4.
-  Definition Const_R5               := Const_R5.
-  Definition Const_R6               := Const_R6.
-  Definition Const_R7               := Const_R7.
-  Definition Const_R8               := Const_R8.
-  Definition Const_R9               := Const_R9.
-  Definition Const_R10              := Const_R10.
-  Definition Const_int64_to_dst_reg := Const_int64_to_dst_reg.
-  Definition Const_int64_to_src_reg := Const_int64_to_src_reg.
-  Definition regmapCompilableType   := regmapCompilableType.
-  Definition Const_eval_regmap      := Const_eval_regmap.
-  Definition Const_upd_regmap       := Const_upd_regmap.
-End Exports.
