comm/rBPFAST.v
@@ -1,0 +1,21 @@
+From Coq Require Import List ZArith.
+Import ListNotations.
+
+From compcert.cfrontend Require Csyntax Ctypes Cop.
+From compcert.common Require Import Values AST Memdata.
+From compcert.lib Require Import Integers.
+
+Definition well_chunk_Z (chunk: memory_chunk):Z := 
+  match chunk with
+  | Mint8unsigned => 1
+  | Mint16unsigned => 2
+  | Mint32 => 4
+  | Mint64 => 8
+  | _ => 10
+  end.
+
+Definition memory_chunk_to_valu32 (chunk: memory_chunk): val := 
+  Vint (Int.repr (well_chunk_Z chunk)). (**r well_chunk implies align_chunk, so we didn't need align_chunk, but we must prove a lemma! *)
+
+Definition memory_chunk_to_valu32_upbound (chunk: memory_chunk): val :=
+  Vint (Int.repr (Int.max_unsigned-(well_chunk_Z chunk))).
