comm/rBPFMemType.v
@@ -1,0 +1,12 @@
+From Coq Require Import List ZArith.
+Import ListNotations.
+
+From compcert.cfrontend Require Csyntax Ctypes Cop.
+From compcert Require Import Integers Values Memtype Memory.
+
+Open Scope Z_scope.
+
+(** permission_eq_eq: permission_eq -> permission_eq -> bool
+  *)
+
+Definition perm_ge (x y: permission): bool := if (Mem.perm_order_dec x y) then true else false.
