equivalence/equivalence.v
@@ -1,0 +1,34 @@
+(**r: equivalence between bpf.model (with formal syntax + semantics) and bpf.src (for dx) *)
+
+From bpf.comm Require Import State Monad.
+From bpf.src Require Import DxInstructions.
+
+From bpf.model Require Import Semantics.
+
+Lemma equivalence_between_formal_and_dx_step:
+  Semantics.step = DxInstructions.step.
+Proof.
+  unfold Semantics.step, DxInstructions.step.
+  unfold DxMonad.bindM, DxMonad.upd_reg, DxMonad.eval_flag, DxMonad.eval_reg, DxMonad.returnM, DxMonad.eval_ins_len, DxMonad.eval_pc, DxMonad.upd_pc_incr, DxMonad.upd_flag, DxMonad.eval_ins.
+  unfold DxIntegers.sint32_t, DxIntegers.int64_t, DxIntegers.int8_t, DxValues.val64_t, DxValues.valu32_t, DxValues.vals32_t.
+Qed.
+
+Lemma equivalence_between_formal_and_dx_aux:
+  forall f,
+    Semantics.bpf_interpreter_aux f = DxInstructions.bpf_interpreter_aux f.
+Proof.
+  unfold Semantics.bpf_interpreter_aux, DxInstructions.bpf_interpreter_aux.
+  unfold DxMonad.bindM, DxMonad.upd_reg, DxMonad.eval_flag, DxMonad.eval_reg, DxMonad.returnM, DxMonad.eval_ins_len, DxMonad.eval_pc, DxMonad.upd_pc_incr, DxMonad.upd_flag.
+  unfold DxIntegers.sint32_t.
+  unfold DxIntegers.int32_0.
+Qed.
+
+Theorem equivalence_between_formal_and_dx:
+  forall f,
+    (**r we should give the register invariant and memory invariant as preconditions? *)
+    Semantics.bpf_interpreter f = DxInstructions.bpf_interpreter f.
+Proof.
+  intros.
+  unfold Semantics.bpf_interpreter, DxInstructions.bpf_interpreter.
+  unfold DxMonad.bindM, DxMonad.upd_reg, DxMonad.eval_flag, DxMonad.eval_reg, DxMonad.returnM.
+Qed.
