model/Semantics.v
@@ -1,0 +1,363 @@
+From compcert Require Import Memory Memtype Integers Values Ctypes AST.
+From Coq Require Import ZArith Lia.
+
+From bpf.comm Require Import Flag Regs State Monad MemRegion rBPFAST rBPFMemType rBPFValues.
+From bpf.model Require Import Syntax Decode.
+
+Open Scope Z_scope.
+Open Scope monad_scope.
+
+
+Definition eval_src (s:reg+imm): M val :=
+  match s with
+  | inl r => eval_reg r
+  | inr i => returnM (Val.longofintu (sint32_to_vint i)) (**r the immediate is always int *)
+  end.
+
+Definition _to_vlong (v: val): val :=
+  match v with
+  | Vlong n => Vlong n (**r Mint64 *)
+  | Vint  n => Vlong (Int64.repr (Int.unsigned n)) (**r Mint8unsigned, Mint16unsigned, Mint32 *) (* (u64) v *)
+  | _       => Vundef
+  end.
+
+Definition vlong_to_vint_or_vlong (chunk: memory_chunk) (v: val): val :=
+  match v with
+  | Vlong n =>
+    match chunk with
+    | Mint8unsigned | Mint16unsigned | Mint32 => Vint (Int.repr (Int64.unsigned n))
+    | Mint64 => Vlong n
+    | _      => Vundef
+    end
+  | _       => Vundef
+  end.
+
+Lemma intu_to_long_intu_eq:
+  forall i j, i = Vint j -> val_intuoflongu (Val.longofintu i) = i.
+Proof.
+  unfold Val.longofintu, val_intuoflongu.
+  intros.
+  rewrite H.
+  assert (H1: Int64.unsigned (Int64.repr (Int.unsigned j)) = Int.unsigned j).
+  - apply Int64.unsigned_repr.
+    assert (Hrange: 0 <= Int.unsigned j <= Int.max_unsigned). { apply Int.unsigned_range_2. }
+    assert (Hmax: Int.max_unsigned <= Int64.max_unsigned).
+    + unfold Int.max_unsigned, Int64.max_unsigned.
+    unfold Int.modulus, Int64.modulus.
+    unfold Int.wordsize, Int64.wordsize.
+    unfold Wordsize_32.wordsize, Wordsize_64.wordsize.
+    simpl.
+    lia.
+    + lia.
+  - rewrite H1.
+    apply f_equal.
+    apply Int.repr_unsigned.
+Qed.
+Close Scope Z_scope.
+
+Definition val_intuoflonguM (vl: val) := returnM (val_intuoflongu vl).
+
+Definition step_alu_binary_operation (a: arch) (bop: binOp) (d :reg) (s: reg+imm): M unit :=
+  do d64 <- eval_reg d;
+  do s64 <- eval_src s;
+  match a with
+  | A32 => 
+    do d32 <- val_intuoflonguM d64;
+    do s32 <- val_intuoflonguM s64; (**r (u32) DST, (u32) SRC/IMM *)
+    match bop with
+    | BPF_ADD  => upd_reg d (Val.longofintu (Val.add  d32 s32))
+    | BPF_SUB  => upd_reg d (Val.longofintu (Val.sub  d32 s32))
+    | BPF_MUL  => upd_reg d (Val.longofintu (Val.mul  d32 s32))
+    | BPF_DIV  => if comp_ne_32 s32 Vzero then (** run-time checking *)
+                    match Val.divu d32 s32 with (**r Val.divu... *)
+                    | Some res => upd_reg d (Val.longofintu res)
+                    | None     => errorM
+                    end
+                  else
+                    upd_flag BPF_ILLEGAL_DIV
+    | BPF_OR   => upd_reg d (Val.longofintu (Val.or   d32 s32))
+    | BPF_AND  => upd_reg d (Val.longofintu (Val.and  d32 s32))
+    | BPF_LSH  => if compu_lt_32 s32 (Vint (Int.repr 32)) then
+                    upd_reg d (Val.longofintu (Val.shl d32 s32))
+                  else
+                    upd_flag BPF_ILLEGAL_SHIFT  (**r if 's' of 'shl d s' is 's > 32', then there is a acceptable error *)
+    | BPF_RSH  => if compu_lt_32 s32 (Vint (Int.repr 32)) then
+                    upd_reg d (Val.longofintu (Val.shru d32 s32))
+                  else
+                    upd_flag BPF_ILLEGAL_SHIFT  (**r if 's' of 'shru d s' is 's > 32', then there is a acceptable error *)
+    | BPF_MOD  => if comp_ne_32 s32 Vzero then (** run-time checking *)
+                    match Val.modu d32 s32 with
+                    | Some res => upd_reg d (Val.longofintu res)
+                    | None     => errorM
+                    end
+                  else
+                    upd_flag BPF_ILLEGAL_DIV
+    | BPF_XOR  => upd_reg d (Val.longofintu (Val.xor  d32 s32))
+    | BPF_MOV  => upd_reg d (Val.longofintu s32)
+    | BPF_ARSH => if compu_lt_32 s32 (Vint (Int.repr 32)) then
+                    upd_reg d (Val.longofintu (Val.shr  d32 s32))
+                  else
+                    upd_flag BPF_ILLEGAL_SHIFT (**r if 's' of 'shr d s' is 's > 32', then there is a acceptable error *)
+    end
+  | A64 =>
+      match bop with
+      | BPF_ADD  => upd_reg d (Val.addl  d64 s64)
+      | BPF_SUB  => upd_reg d (Val.subl  d64 s64)
+      | BPF_MUL  => upd_reg d (Val.mull  d64 s64)
+      | BPF_DIV  => if compl_ne s64 val64_zero then (** run-time checking *)
+                      match Val.divlu d64 s64 with (**r run-time checking *)
+                      | Some res => upd_reg d res
+                      | None     => errorM
+                      end
+                    else
+                      upd_flag BPF_ILLEGAL_DIV
+      | BPF_OR   => upd_reg d (Val.orl   d64 s64)
+      | BPF_AND  => upd_reg d (Val.andl  d64 s64)
+      (**r we must do type-checking of 's64' first, to ensure it is exactly 'vint' *)
+      | BPF_LSH  => if complu_lt (val_intuoflongu s64) (Vlong (Int64.repr 64)) then
+                      upd_reg d (Val.shll d64 s64)
+                    else
+                      upd_flag BPF_ILLEGAL_SHIFT  (**r if 's' of 'shl d s' is 's > 64', then there is a acceptable error *)
+      | BPF_RSH  => if complu_lt (val_intuoflongu s64) (Vlong (Int64.repr 64)) then
+                      upd_reg d (Val.shrlu d64 s64)
+                    else
+                      upd_flag BPF_ILLEGAL_SHIFT  (**r if 's' of 'shr d s' is 's > 64', then there is a acceptable error *)
+      | BPF_MOD  => if compl_ne s64 val64_zero then (** run-time checking *)
+                      match Val.modlu d64 s64 with (**r run-time checking *)
+                      | Some res => upd_reg d res
+                      | None     => errorM
+                      end
+                    else
+                      upd_flag BPF_ILLEGAL_DIV
+(**r to avoid translate option type to C, the refinement version defines a new division:
+Definition val64_divlu (x y: val): val :=
+  match Val.divlu x y with
+  | Some res => res
+  | None => Vundef
+  end.
+And the semantics function does:
+  | op_BPF_DIV64   =>
+    if compl_ne src64 val64_zero then
+      do _ <- upd_reg dst (val64_divlu dst64 src64);
+        upd_flag BPF_OK
+    else
+      upd_flag BPF_ILLEGAL_DIV
+
+ *)
+      | BPF_XOR  => upd_reg d (Val.xorl  d64 s64)
+      | BPF_MOV  => upd_reg d s64
+      | BPF_ARSH => if complu_lt (val_intuoflongu s64) (Vlong (Int64.repr 64)) then
+                      upd_reg d (Val.shrl d64 s64)
+                    else
+                      upd_flag BPF_ILLEGAL_SHIFT  (**r if 's' of 'shru d s' is 's > 64', then there is a acceptable error? *)
+      end
+  end.
+
+Definition step_branch_cond (c: cond) (d: reg) (s: reg+imm): M bool :=
+  do dst <- eval_reg d;
+  do src <- eval_src s;
+  returnM (match c with
+  | Eq  => compl_eq   dst src
+  | SEt => complu_set dst src
+  | Ne  => compl_ne   dst src
+  | Gt sign => 
+    match sign with
+    | Unsigned => complu_gt dst src
+    | Signed   => compl_gt  dst src
+    end
+  | Ge sign =>
+    match sign with
+    | Unsigned => complu_ge dst src
+    | Signed   => compl_ge  dst src
+    end
+  | Lt sign => 
+    match sign with
+    | Unsigned => complu_lt dst src
+    | Signed   => compl_lt  dst src
+    end
+  | Le sign => 
+    match sign with
+    | Unsigned => complu_le dst src
+    | Signed   => compl_le  dst src
+    end
+  end).
+
+Definition get_mem_region (n:nat): M memory_region :=
+  do mrs      <- eval_mrs_regions;
+  returnM (MyMemRegionsIndexnat mrs n).
+
+Definition get_add (x y: val): M val := returnM (Val.add x y).
+
+Definition get_sub (x y: val): M val := returnM (Val.sub x y).
+
+Definition get_addr_ofs (x: val) (ofs: int): M val := returnM (val_intuoflongu (Val.addl x (Val.longofint (sint32_to_vint ofs)))).
+
+Definition get_block_ptr (mr: memory_region) : M val := returnM (block_ptr mr).
+
+Definition get_start_addr (mr: memory_region): M val := returnM (start_addr mr).
+
+Definition get_block_size (mr: memory_region): M val := returnM (block_size mr).
+
+Definition get_block_perm (mr: memory_region): M permission := returnM (block_perm mr).
+
+Definition is_well_chunk_bool (chunk: memory_chunk) : M bool :=
+  match chunk with
+  | Mint8unsigned | Mint16unsigned | Mint32 | Mint64 => returnM true
+  | _ => returnM false
+  end.
+
+Definition check_mem_aux2 (mr: memory_region) (perm: permission) (addr: val) (chunk: memory_chunk): M val :=
+  do well_chunk <- is_well_chunk_bool chunk;
+    if well_chunk then
+      do ptr    <- get_block_ptr mr; (**r Vptr b 0 *)
+      do start  <- get_start_addr mr;
+      do size   <- get_block_size mr;
+      do lo_ofs <- get_sub addr start;
+      do hi_ofs <- get_add lo_ofs (memory_chunk_to_valu32 chunk);
+        if (andb (compu_le_32 Vzero lo_ofs) (compu_lt_32 hi_ofs size)) then
+          if (andb (compu_le_32 lo_ofs (memory_chunk_to_valu32_upbound chunk))
+                   (comp_eq_32 Vzero (val32_modu lo_ofs (memory_chunk_to_valu32 chunk)))) then
+            do mr_perm  <- get_block_perm mr;
+              if (perm_ge mr_perm perm) then
+                returnM (Val.add ptr lo_ofs) (**r Vptr b lo_ofs *)
+              else
+                returnM Vnullptr
+          else
+            returnM Vnullptr (**r = 0 *)
+        else
+          returnM Vnullptr
+    else
+      returnM Vnullptr.
+
+Fixpoint check_mem_aux (num: nat) (perm: permission) (chunk: memory_chunk) (addr: val) {struct num}: M val :=
+  match num with
+  | O => returnM Vnullptr
+  | S n =>
+    do cur_mr   <- get_mem_region n;
+    do check_mem <- check_mem_aux2 cur_mr perm addr chunk;
+      if comp_eq_ptr8_zero check_mem then
+        check_mem_aux n perm chunk addr
+      else
+        returnM check_mem
+  end.
+
+Definition check_mem (perm: permission) (chunk: memory_chunk) (addr: val): M val :=
+  do well_chunk <- is_well_chunk_bool chunk;
+    if well_chunk then
+      do mem_reg_num <- eval_mrs_num;
+      do check_mem <- check_mem_aux mem_reg_num perm chunk addr;
+        if comp_eq_ptr8_zero check_mem then
+          returnM Vnullptr
+        else
+          returnM check_mem
+    else
+      returnM Vnullptr.
+
+Definition step_load_x_operation (chunk: memory_chunk) (d:reg) (s:reg) (ofs:off): M unit :=
+  do m    <- eval_mem;
+  do mrs  <- eval_mem_regions;
+  do sv   <- eval_reg s;
+  do addr <- get_addr_ofs sv ofs;
+  do ptr  <- check_mem Readable chunk addr;
+    if comp_eq_ptr8_zero ptr then
+      upd_flag BPF_ILLEGAL_MEM
+    else
+      do v <- load_mem chunk ptr;
+      do _ <- upd_reg d v;
+        upd_flag BPF_OK
+.
+
+Definition step_store_operation (chunk: memory_chunk) (d: reg) (s: reg+imm) (ofs: off): M unit :=
+  do m    <- eval_mem;
+  do mrs  <- eval_mem_regions;
+  do dv   <- eval_reg d;
+  do addr <- get_addr_ofs dv ofs;
+  do ptr  <- check_mem Writable chunk addr;
+    if comp_eq_ptr8_zero ptr then
+      upd_flag BPF_ILLEGAL_MEM
+    else
+      match s with
+      | inl r =>
+        do src <- eval_reg r;
+        do _ <- store_mem_reg chunk ptr src;
+          upd_flag BPF_OK
+      | inr i =>
+        do _ <- store_mem_imm chunk ptr (Val.longofintu (sint32_to_vint i));
+          upd_flag BPF_OK
+      end
+.
+
+Definition decodeM (i: int64) : M instruction := returnM (decode i).
+Definition get_immediate (ins:int64):M int := returnM (get_immediate ins).
+
+Definition step : M unit :=
+  do pc   <- eval_pc;
+  do ins64<- eval_ins pc;
+  do ins  <- decodeM ins64;
+    match ins with
+    | BPF_NEG a d =>
+      match a with
+      | A32 => do d32 <- eval_reg d;
+                 upd_reg d (Val.longofintu (Val.neg (val_intuoflongu d32)))
+      | A64 => do d64 <- eval_reg d;
+                 upd_reg d (Val.negl d64)
+      end
+
+    | BPF_BINARY a bop d s =>
+      step_alu_binary_operation a bop d s
+
+    | BPF_JA ofs => upd_pc (Int.add pc ofs)
+    | BPF_JUMP c d s ofs =>
+      do cond <- step_branch_cond c d s;
+      if cond then
+        upd_pc (Int.add pc ofs)
+      else
+        upd_flag BPF_OK
+    | BPF_LDDW d i =>
+      do len  <- eval_ins_len;
+        if (Int.lt (Int.add pc Int.one) len) then (**r pc+1 < len: pc+1 is less than the length of l *)
+          do next_ins <- eval_ins (Int.add pc Int.one);
+          do next_imm <- get_immediate next_ins;
+          do _ <- upd_reg d (Val.or (Val.longofint (sint32_to_vint i)) (Val.shl  (Val.longofint (sint32_to_vint next_imm)) (sint32_to_vint (Int.repr 32))));
+          do _ <- upd_pc_incr;
+            upd_flag BPF_OK
+        else
+          upd_flag BPF_ILLEGAL_LEN
+    | BPF_LDX chunk d s ofs =>
+      step_load_x_operation chunk d s ofs
+    | BPF_ST chunk d s ofs =>
+      step_store_operation chunk d s ofs
+
+    | BPF_RET => upd_flag BPF_SUCC_RETURN
+    | BPF_ERR => upd_flag BPF_ILLEGAL_INSTRUCTION
+    end.
+
+Fixpoint bpf_interpreter_aux (fuel: nat) {struct fuel}: M unit :=
+  match fuel with
+  | O => upd_flag BPF_ILLEGAL_LEN
+  | S fuel0 =>
+    do len  <- eval_ins_len;
+    do pc <- eval_pc;
+      if(andb (Int_le Int.zero pc) (Int.lt pc len)) then (**r 0 < pc < len: pc is less than the length of l *)
+        do _ <- step;
+        do _ <- upd_pc_incr;
+        do f <- eval_flag;
+          if flag_eq f BPF_OK then
+            bpf_interpreter_aux fuel0
+          else
+            returnM tt
+      else
+        upd_flag BPF_ILLEGAL_LEN
+  end.
+
+Definition bpf_interpreter (fuel: nat): M val :=
+  do bpf_ctx  <- get_mem_region 0;
+  do _        <- upd_reg R1 (start_addr bpf_ctx); (**r let's say the ctx memory region is also be the first one *)
+  do _        <- bpf_interpreter_aux fuel;
+  do f        <- eval_flag;
+    if flag_eq f BPF_SUCC_RETURN then
+      eval_reg R0
+    else
+      returnM val64_zero.
+
+Close Scope monad_scope.
