model/Syntax.v
@@ -1,0 +1,45 @@
+From compcert Require Import Ctypes AST Integers.
+
+From bpf.comm Require Import Int16 Regs.
+
+(** For use to distinguish ALU32 and ALU64 *)
+Inductive arch := A32 | A64.
+
+(** For condition flags *)
+(*Inductive signedness := Signed | Unsigned.*)
+
+Inductive cond := 
+  Eq 
+| Gt: signedness -> cond 
+| Ge: signedness -> cond
+| Lt: signedness -> cond
+| Le: signedness -> cond
+| SEt 
+| Ne
+.
+
+Definition off := int.
+Definition imm := int.
+
+Inductive binOp: Type :=
+  BPF_ADD | BPF_SUB | BPF_MUL | BPF_DIV | BPF_OR | BPF_AND
+| BPF_LSH | BPF_RSH | BPF_MOD | BPF_XOR | BPF_MOV| BPF_ARSH.
+
+Inductive instruction: Type :=
+  (**r ALU64/32*)
+  | BPF_NEG    : arch -> reg -> instruction
+  | BPF_BINARY : arch -> binOp -> reg -> reg+imm -> instruction  
+  (**r Branch *)
+  | BPF_JA  : off -> instruction
+  | BPF_JUMP: cond -> reg -> reg+imm -> off -> instruction
+
+  (**r Load *)
+  | BPF_LDDW   : reg -> imm -> instruction
+  (**r Load_x *)
+  | BPF_LDX : memory_chunk -> reg -> reg -> off -> instruction
+  (**r Store/ Store_x *)
+  | BPF_ST  : memory_chunk -> reg -> reg+imm -> off -> instruction
+  (**r exit *)
+  | BPF_RET  : instruction
+  | BPF_ERR  : instruction
+.
