proof/CommonLemma.v
@@ -1,5 +1,5 @@
 From compcert Require Import Coqlib Clight Integers Values Ctypes Memory.
-From bpf.src Require Import DxRegs DxState DxMonad.
+From bpf.comm Require Import Regs State.
 From bpf.proof Require Import Clightlogic CommonLib.
 (* From Ltac2 Require Import Ltac2 Message. *)
 From Coq Require Import List Lia ZArith.
@@ -663,11 +663,11 @@ Qed.
 Lemma upd_reg_preserves_perm: forall r vl vl' chunk st m1 m m2 b b' ofs ofs' k p
   (Hstate_inject: Mem.inject inject_id (bpf_m st) m) (**r (inject_bl_state b') *)
   (Hstore: Mem.store chunk m b' ofs' vl' = Some m2)
-  (Hrbpf_m: bpf_m (DxState.upd_reg r vl st) = m1)
+  (Hrbpf_m: bpf_m (upd_reg r vl st) = m1)
   (Hrbpf_perm: Mem.perm m1 b ofs k p),
     Mem.perm m2 b ofs k p.
 Proof.
-    unfold DxState.upd_reg; simpl; intros; subst.
+    unfold upd_reg; simpl; intros; subst.
     apply Mem.perm_inject with (f:= inject_id) (m2:=m) (b2:= b) (delta:=0%Z)in Hrbpf_perm.
     rewrite Z.add_0_r in Hrbpf_perm.
     apply (Mem.perm_store_1 _ _ _ _ _ _ Hstore _ _ _ _ Hrbpf_perm).
